Source/IntegrationTests/TestFiles/LitTests/LitTest/reveal/revealFunctions.dfy
@@ -1,0 +1,83 @@
+// RUN: ! %verify --type-system-refresh --allow-axioms --bprint:%t.bpl --isolate-assertions --boogie "/printPruned:%S/pruned" %s > %t
+// RUN: %diff "%s.expect" "%t"
+
+function P(): bool {
+  true
+}
+
+blind method Foo()
+{
+  if (*) {
+    reveal P;
+    assert P();
+  } else {
+    assert P(); // error
+  }
+}
+
+blind function Zer(): int {
+  Q() // requires error
+}
+
+blind function Zaz(): int {
+  reveal P; 
+  Q()
+}
+
+function Q(): int 
+  requires P() {
+  3
+}
+
+function EnsuresFuncFoo(): bool
+  ensures EnsuresFuncFoo()
+
+blind method UseEnsuresFuncFoo() {
+  if (*) {
+    reveal EnsuresFuncFoo;
+    assert EnsuresFuncFoo();
+  } else {
+    assert EnsuresFuncFoo(); // no error. Could be changed in the future
+  }
+}
+
+opaque predicate OpaqueFunc() {
+  true
+}
+
+blind method OpaqueUser() {
+  if (*) {
+    reveal OpaqueFunc;
+    assert OpaqueFunc();
+  } else {
+    assert OpaqueFunc(); // error
+  }
+}
+
+blind method FunctionSubsetResult() {
+    var x: nat := Natty();
+    assert x >= 0; // no error
+}
+
+function Natty(): nat {
+  3
+}
+class O { var x: int }
+function Obj(o: O): int 
+  ensures Obj(o) > 0
+{
+  3
+}
+
+blind method ReadsClause() {
+  var o := new O;
+  var before := Obj(o);
+  o.x := 3;
+  if (*) {
+    assert Obj(o) == before; // passes, because reads clause is never hidden
+  } else {
+    assert Obj(o) == before by { // passes
+      reveal Obj;
+    }
+  }
+}
