Source/IntegrationTests/TestFiles/LitTests/LitTest/reveal/revealInExpression.dfy
@@ -1,0 +1,21 @@
+// echo ''
+// NORUN: ! %verify --type-system-refresh --allow-axioms --bprint:%t.bpl --isolate-assertions --boogie "/printPruned:%S/pruned" %s > %t
+// NORUN: %diff "%s.expect" "%t"
+
+function P(): bool {
+  true
+}
+
+function Q(): int 
+  requires P() {
+  3
+}
+
+blind method RevealExpressionScope()
+{
+  reveal P;
+  reveal Q;
+  assert Q() == 3;
+  assert reveal P; reveal Q; Q() == 3;
+  assert P();
+}
