Source/IntegrationTests/TestFiles/LitTests/LitTest/reveal/revealMethods.dfy
@@ -1,0 +1,25 @@
+// echo ''
+// NoRUN: ! %verify --type-system-refresh --allow-axioms --bprint:%t.bpl --isolate-assertions --boogie "/printPruned:%S/pruned" %s > %t
+// NoRUN: %diff "%s.expect" "%t"
+
+blind method MethodEnsuresAreHidden() {
+  // var x := Bar();
+  // if (*) {
+  //   reveal Bar();
+  //   assert x;
+  // } else {
+  //   assert x; // error
+  // }
+  // assert x;
+}
+
+method Bar() returns (x: bool) 
+  ensures x
+
+// Consequence axiom also contains information about subset types of the return types
+// Reveals in contracts are fine, but they never escape the contract.
+
+// Add an option 
+// TODO what to do with reveals in contracts?
+// TODO add test cases that see how blindness interops with contracts of the blind callable
+// TODO if a contract has reveals clauses, do they get copied to the caller?
