Source/IntegrationTests/TestFiles/LitTests/LitTest/reveal/revealSubsets.dfy
@@ -1,0 +1,30 @@
+// echo ''
+// NoRUN: ! %verify --type-system-refresh --allow-axioms --bprint:%t.bpl --isolate-assertions --boogie "/printPruned:%S/pruned" %s > %t
+// NoRUN: %diff "%s.expect" "%t"
+
+function P(): bool {
+  true
+}
+
+function Q(): int 
+  requires P() {
+  3
+}
+
+blind method FunctionSubsetResult(a: nat) {
+  assert a >= 0;
+  if (*) { 
+    var x: nat := Natty();
+    assert x >= 0;
+  } else if (*) {
+    var y: int := Natty();
+    assert y >= 0;
+  } else {
+    reveal Natty;
+    var z: nat := Natty();
+    assert z >= 0;
+  }
+}
+function Natty(): nat {
+  3
+}
